FOL/NV/Sub/Var/All/Ind/Sub.lean
@@ -129,7 +129,7 @@ def IsSub (σ : VarName → VarName) (F F' : Formula) : Prop := IsSubAux σ ∅ 
 theorem substitution_theorem_aux
   (D : Type)
   (I : Interpretation D)
-  (V V' : VarAssignment D)
+  (V V' : Assignment D)
   (E : Env)
   (σ : VarName → VarName)
   (binders : Finset VarName)
@@ -276,7 +276,7 @@ theorem substitution_theorem_aux
 theorem substitution_theorem
   (D : Type)
   (I : Interpretation D)
-  (V : VarAssignment D)
+  (V : Assignment D)
   (E : Env)
   (σ : VarName → VarName)
   (F F' : Formula)
