FOL/NV/Sub/Var/One/Rec/Admits.lean
@@ -998,7 +998,7 @@ theorem admitsAux_isFreeIn
 theorem substitution_theorem_aux
   (D : Type)
   (I : Interpretation D)
-  (V V' : VarAssignment D)
+  (V V' : Assignment D)
   (E : Env)
   (v t : VarName)
   (binders : Finset VarName)
@@ -1136,7 +1136,7 @@ theorem substitution_theorem_aux
 theorem substitution_theorem
   (D : Type)
   (I : Interpretation D)
-  (V : VarAssignment D)
+  (V : Assignment D)
   (E : Env)
   (v t : VarName)
   (F : Formula)
